theories/Dot/examples/positive_div.v
@@ -65,7 +65,7 @@ Section helpers.
   Lemma wp_nge m n (Hnge : ¬ m > n) : ⊢ WP m > n {{ w, w ≡ false }}.
   Proof. wp_bin. ev; simplify_eq/=. case_decide; by [|lia]. Qed.
 
-  Lemma setp_value Γ (T : olty Σ 0) v: Γ s⊨ v : T ⊣⊢ (□∀ ρ, s⟦ Γ ⟧* ρ → T vnil ρ v.[ρ]).
+  Lemma setp_value Γ (T : olty Σ 0) v: Γ s⊨ v : T ⊣⊢ (□∀ ρ, sG⟦ Γ ⟧* ρ → T vnil ρ v.[ρ]).
   Proof.
     rewrite /=; properness => //; iSplit;
       [rewrite wp_value_inv|rewrite -wp_value]; iIntros "#$".
